finished the removal of symbols for arbitrary signatures with finitely many term symbols or else discreteness of the the type of term symbols

theories/TRAKHTENBROT/Sig_rem_syms.v
@@ -16,9 +16,16 @@ From Undecidability.Shared.Libs.DLW.Vec
   Require Import pos vec.
 
 From Undecidability.TRAKHTENBROT
-  Require Import notations fol_ops utils fo_terms fo_logic.
+  Require Import notations fol_ops utils fo_terms fo_logic fo_sat.
 
 Set Implicit Arguments.
+
+Fact in_concat_iff X (ll : list (list X)) x : In x (concat ll) <-> exists l, In x l /\ In l ll.
+Proof.
+  rewrite <- (map_id ll) at 1.
+  rewrite <- flat_map_concat_map, in_flat_map.
+  firstorder.
+Qed.
 
 Local Notation ø := vec_nil.
 
@@ -58,38 +65,88 @@ Section Sig_remove_symbols.
 
   Section removing_symbols.
 
-    Let rem_syms (t : 𝕋) : 
-        { A : 𝔽' | forall X M φ ψ, 
-                          (forall n, φ n = ψ (S n))
-                       -> ψ 0 = fo_term_sem (fom_syms M) φ t 
-                      <-> fol_sem (@fom_nosyms X M) ψ A }.
+    Let f k (p : pos k) n : 𝕋' := match n with 0 => £ (pos2nat p) | S n => £ (n+1+k) end.
+
+    Definition fot_rem_syms : 𝕋 -> 𝔽'.
+    Proof.
+      induction 1 as [ n | s v w ] using fo_term_recursion.
+      + exact (fol_atom Σ' e (£0##£(S n)##ø)).
+      + exact (let A  := fol_atom Σ' (inl s) (£(ar_syms _ s)##vec_set_pos (fun p => £ (pos2nat p))) in
+               let wB := vec_set_pos (fun p => (vec_pos w p)⦃f p⦄) 
+               in fol_mquant fol_ex (ar_syms _ s) (A ⟑ fol_vec_fa wB)).
+    Defined.
+
+    Local Fact fot_rem_syms_fix0 n : fot_rem_syms (in_var n) = fol_atom Σ' e (£0##£(S n)##ø).
+    Proof. apply fo_term_recursion_fix_0. Qed.
+
+    Local Fact fot_rem_syms_fix1 s v : 
+                 fot_rem_syms (in_fot s v) 
+               = let A  := fol_atom Σ' (inl s) (£(ar_syms _ s)##vec_set_pos (fun p => £ (pos2nat p))) in
+                 let wB := vec_set_pos (fun p => (fot_rem_syms (vec_pos v p))⦃f p⦄) 
+                 in fol_mquant fol_ex (ar_syms _ s) (A ⟑ fol_vec_fa wB).
+    Proof.
+      unfold fot_rem_syms at 1.
+      rewrite fo_term_recursion_fix_1.
+      do 3 f_equal.
+      apply vec_pos_ext; intros; rew vec.
+    Qed.
+
+    Fact fot_rem_syms_rels t : incl (fol_rels (fot_rem_syms t)) (inr (inl tt)::map inl (fo_term_syms t)).
     Proof.
       induction t as [ n | s v IHv ] using fo_term_pos_rect.
-      + exists (fol_atom Σ' e (£0##£(S n)##ø)).
-        intros X (sy,re) phi psi H2; simpl.
-        rewrite <- H2; tauto.
-      + apply vec_reif_t in IHv.
-        destruct IHv as (vB & HB).
-        set (A := fol_atom Σ' (inl s) (£(ar_syms _ s)##vec_set_pos (fun p => £ (pos2nat p)))).
-        set (f (p : pos (ar_syms _ s)) n := match n with 0 => £ (pos2nat p) | S n => £ (n+1+ar_syms _ s) end : 𝕋').
-        set (wB := vec_set_pos (fun p => (vec_pos vB p)⦃f p⦄)).
-        exists (fol_mquant fol_ex (ar_syms _ s) (A ⟑ fol_vec_fa wB)).
-        intros X M phi psi H2; simpl.
-        specialize (fun p => HB p X M).
-        destruct M as (sy,re).
+      + rewrite fot_rem_syms_fix0; cbv; tauto.
+      + rewrite fot_rem_syms_fix1; simpl.
+        rewrite fol_rels_mquant; simpl.
+        unfold fol_vec_fa, fol_lconj.
+        rewrite fol_rels_bigop.
+        intros r; simpl.
+        rewrite in_app_iff, in_flat_map.
+        intros [ <- | [ H | [] ] ]; auto; revert H.
+        intros (A & H1 & H2); revert H2.
+        apply vec_list_inv in H1.
+        destruct H1 as (p & ->); rew vec.
+        rewrite fol_rels_subst.
+        intros H; apply IHv in H; revert H.
+        simpl; rewrite in_map_iff.
+        intros [ <- | (s' & <- & Hs') ]; auto.
+        do 2 right.
+        rewrite in_map_iff; exists s'; split; auto.
+        rewrite in_concat_iff.
+        exists (fo_term_syms (vec_pos v p)); split; auto.
+        rewrite <- vec_map_set_pos, vec_list_vec_map, in_map_iff.
+        exists (vec_pos v p); split; auto.
+        apply in_vec_list.
+        replace (vec_set_pos (vec_pos v)) with v.
+        * apply in_vec_pos.
+        * apply vec_pos_ext; intros; rew vec.
+    Qed.
+ 
+    Fact fot_rem_syms_spec t X M φ ψ : 
+            (forall n, φ n = ψ (S n))
+         -> ψ 0 = fo_term_sem (fom_syms M) φ t 
+        <-> fol_sem (@fom_nosyms X M) ψ (fot_rem_syms t).
+    Proof.
+      revert X M φ ψ.
+      induction t as [ n | s v IHv ] using fo_term_pos_rect; 
+        intros X M phi psi H2.
+      + destruct M as (re,sy); simpl; rewrite <- H2; tauto.
+      + specialize (fun p => IHv p X M).
+        rewrite fot_rem_syms_fix1.
+        destruct M as (sy,re); simpl.
         rewrite fol_sem_mexists.
         split.
         * intros H3.
           exists (vec_set_pos (fun p => fo_term_sem sy phi (vec_pos v p))); split.
-          - unfold A, fom_nosyms; simpl.
+          - simpl. 
             replace (ar_syms _ s) with (0+ar_syms _ s) at 3 by lia.
             rewrite env_vlift_fix1; simpl; f_equal; rewrite H3; simpl; f_equal.
             apply vec_pos_ext; intros p; rew vec; rew fot.
             rewrite env_vlift_fix0; rew vec.
-          - rewrite fol_sem_vec_fa; intros p.
-            unfold wB; rew vec.
+          - simpl.
+            rewrite fol_sem_vec_fa; intros p.
+            rew vec.
             rewrite fol_sem_subst.
-            rewrite <- HB; auto.
+            rewrite <- IHv; auto.
             2: reflexivity.
             simpl; rew fot.
             rewrite env_vlift_fix0; rew vec.
@@ -97,93 +154,306 @@ Section Sig_remove_symbols.
             replace (n+1+ar_syms _ s) with ((S n)+ar_syms _ s) by lia.
             rewrite env_vlift_fix1; auto.
         * intros (w & Hw1 & Hw2).
-          unfold A in Hw1; simpl in Hw1.
+          simpl in Hw1.
           replace (ar_syms _ s) with (0+ar_syms _ s) in Hw1 at 2 by lia.
           rewrite env_vlift_fix1 in Hw1.
           rewrite Hw1; clear Hw1.
           simpl; f_equal.
           apply vec_pos_ext; intros p; rew vec.
           rew fot.
-          unfold wB in Hw2.
           rewrite fol_sem_vec_fa in Hw2.
           specialize (Hw2 p); revert Hw2; rew vec; intros Hw2.
           rewrite fol_sem_subst in Hw2.
-          rewrite <- HB with (φ := phi) in Hw2; auto.
+          rewrite <- IHv with (φ := phi) in Hw2; auto.
           intros n; simpl.
           replace (n+1+ar_syms _ s) with ((S n)+ar_syms _ s) by lia.
           rewrite env_vlift_fix1; auto.
     Qed.
 
-    Definition fot_rem_syms t := proj1_sig (rem_syms t).
-
-    Fact fot_rem_syms_spec t X M φ ψ : 
-            (forall n, φ n = ψ (S n))
-         -> ψ 0 = fo_term_sem (fom_syms M) φ t 
-        <-> fol_sem (@fom_nosyms X M) ψ (fot_rem_syms t).
-    Proof. apply (proj2_sig (rem_syms t)). Qed. 
- 
   End removing_symbols.
 
   Section now_formulas.
 
-    Let rem_syms (A : 𝔽) : 
-        { A' : 𝔽' | forall X M φ, 
-                          fol_sem M φ A 
-                      <-> fol_sem (@fom_nosyms X M) φ A' }.
+    Let f k (p : pos k) n : 𝕋' := match n with 0 => £ (pos2nat p) | S n => £ (n+k) end.
+
+    Fixpoint fol_rem_syms A : 𝔽' :=
+      match A with
+        | ⊥               => ⊥
+        | fol_atom _ r v  => let A  := fol_atom Σ' (inr (inr r)) (vec_set_pos (fun p => £ (pos2nat p))) in
+                             let wB := vec_set_pos (fun p => (fot_rem_syms (vec_pos v p))⦃f p⦄)
+                             in  fol_mquant fol_ex (ar_rels _ r) (A ⟑ fol_vec_fa wB)
+        | fol_bin c A B   => fol_bin c (fol_rem_syms A) (fol_rem_syms B)
+        | fol_quant q A   => fol_quant q (fol_rem_syms A)
+      end.
+
+    Fact fol_rem_syms_rels A : incl (fol_rels (fol_rem_syms A))
+                                    (inr (inl tt) :: map inl (fol_syms A) ++ map (fun r => inr (inr r)) (fol_rels A)).
     Proof.
-      induction A as [ | r v | b A (A' & HA') B (B' & HB') | q A (A' & HA') ].
-      + exists ⊥; simpl; tauto.
-      + set (vB := vec_map fot_rem_syms v).
-        set (A := fol_atom Σ' (inr (inr r)) (vec_set_pos (fun p => £ (pos2nat p)))).
-        set (f (p : pos (ar_rels _ r)) n := match n with 0 => £ (pos2nat p) | S n => £ (n+ar_rels _ r) end : 𝕋').
-        set (wB := vec_set_pos (fun p => (fot_rem_syms (vec_pos v p))⦃f p⦄)).
-        exists (fol_mquant fol_ex (ar_rels _ r) (A ⟑ fol_vec_fa wB)).
-        intros X (sy,re) phi; rewrite fol_sem_mexists; split.
-        * intros H; simpl in H.
-          exists (vec_map (fo_term_sem sy phi) v); split.
-          - unfold A; simpl.
-            revert H; apply fol_equiv_ext; f_equal.
+      induction A as [ | r v | b A IHA B IHB | q A IHA ].
+      + cbv; tauto.
+      + simpl.
+        rewrite fol_rels_mquant; simpl.
+        unfold fol_vec_fa, fol_lconj.
+        rewrite fol_rels_bigop.
+        intros s; simpl; rewrite in_app_iff, in_flat_map, in_app_iff.
+        intros [ <- | [ (A & H1 & H2) | [] ] ]; simpl; auto; revert H2.
+        apply vec_list_inv in H1; destruct H1 as (p & ->); rew vec; intros H1.
+        rewrite fol_rels_subst in H1.
+        apply fot_rem_syms_rels in H1; simpl in H1.
+        rewrite in_map_iff in H1.
+        destruct H1 as [ | (s' & <- & H1) ]; auto.
+        right; left; apply in_map_iff.
+        exists s'; split; auto.
+        apply in_flat_map.
+        exists (vec_pos v p); split; auto.
+        apply in_vec_list, in_vec_pos.
+      + intros r; simpl.
+        repeat rewrite map_app.
+        repeat rewrite in_app_iff.
+        intros [ H | H ].
+        * apply IHA in H; revert H; simpl.
+          rewrite in_app_iff; tauto.
+        * apply IHB in H; revert H; simpl.
+          rewrite in_app_iff; tauto.
+      + intros r; simpl.
+        repeat rewrite map_app.
+        repeat rewrite in_app_iff.
+        intros H; apply IHA in H; revert H.
+        simpl; rewrite in_app_iff; tauto.
+    Qed.
+    
+    Fact fol_rem_syms_spec A X M φ : 
+           fol_sem M φ A 
+       <-> fol_sem (@fom_nosyms X M) φ (fol_rem_syms A).
+    Proof.
+      revert φ.
+      induction A as [ | r v | b A IHA B IHB | q A IHA ]; intros phi.
+      + simpl; tauto.
+      + simpl; rewrite fol_sem_mexists; split.
+        * intros H; simpl in H |- *.
+          exists (vec_map (fo_term_sem (fom_syms M) phi) v); split.
+          - revert H; apply fol_equiv_ext.
+            unfold fom_nosyms; destruct M as (re,sy); simpl; f_equal.
             apply vec_pos_ext; intros p; rew vec; rew fot.
             rewrite env_vlift_fix0; rew vec.
-          - rewrite fol_sem_vec_fa; intros p.
-            unfold wB; rew vec.
-            rewrite fol_sem_subst.
+          - rewrite fol_sem_vec_fa; intros p; rew vec.
+            rewrite fol_sem_subst; simpl.
             rewrite <- fot_rem_syms_spec; auto.
             2: intro; reflexivity.
             simpl.
             rewrite env_vlift_fix0; rew vec.
             apply fo_term_sem_ext.
             intros; rewrite env_vlift_fix1; auto.
-        * intros (w & Hw1 & Hw2).
-          unfold A in Hw1; simpl in Hw1.
-          simpl; revert Hw1; apply fol_equiv_ext; f_equal.
+        * intros (w & Hw1 & Hw2); revert Hw1.
+          simpl; apply fol_equiv_ext.
+          unfold fom_nosyms; destruct M as (re,sy); simpl; f_equal.
           apply vec_pos_ext; intros p; rew vec; rew fot.
           rewrite env_vlift_fix0.
           rewrite fol_sem_vec_fa in Hw2.
-          specialize (Hw2 p); revert Hw2; unfold wB; rew vec.
+          specialize (Hw2 p); revert Hw2; rew vec.
           rewrite fol_sem_subst, <- fot_rem_syms_spec; auto.
           2: intro; reflexivity.
           simpl; rewrite env_vlift_fix0.
           intros ->; apply fo_term_sem_ext.
           intros; rewrite env_vlift_fix1; auto.
-      + exists (fol_bin b A' B').  
-        intros X M phi; simpl.
-        apply fol_bin_sem_ext; auto.
-      + exists (fol_quant q A').
-        intros X M phi.
-        simpl; apply fol_quant_sem_ext.
+      + simpl; apply fol_bin_sem_ext; auto.
+      + simpl; apply fol_quant_sem_ext.
         intro; auto.
     Qed.
 
-    Definition fol_rem_syms A := proj1_sig (rem_syms A).
-
-    Fact fol_rem_syms_spec A X M φ : 
-           fol_sem M φ A 
-       <-> fol_sem (@fom_nosyms X M) φ (fol_rem_syms A).
-    Proof. apply (proj2_sig (rem_syms A)). Qed.
-
   End now_formulas.
 
-  Check fol_rem_syms_spec.
+  Variable (X : Type) (M : fo_model Σ' X) (HM : fom_rels M e = rel2_on_vec eq).
+
+  Definition fol_rel_fun (s : syms Σ) : 𝔽' := 
+       let n := ar_syms _ s
+       in ∀∀ fol_mquant fol_fa n (   
+              fol_atom Σ' (inl s) (£(S n)##vec_set_pos (fun p => £(pos2nat p))) 
+                     ⤑ fol_atom Σ' (inl s) (£n##vec_set_pos (fun p => £(pos2nat p)))
+                     ⤑ fol_atom _ e (£(S n)##£n##ø) ).
+
+  Fact fol_rel_fun_spec s φ : fol_sem M φ (fol_rel_fun s)  <-> graph_fun (fun v x => fom_rels M (inl s) (x##v)).
+  Proof.
+    unfold fol_rel_fun; simpl; split.
+    + intros H v x y H1 H2.
+      specialize (H x y).
+      rewrite fol_sem_mforall in H.
+      specialize (H v); simpl fol_sem in H.
+      rewrite env_vlift_fix1 with (k := 1) in H.
+      rewrite env_vlift_fix1 with (k := 0) in H.
+      rewrite HM in H; simpl in H.
+      apply H.
+      * revert H1; apply fol_equiv_ext; do 2 f_equal.
+        apply vec_pos_ext; intros p; rew vec; rew fot.
+        rewrite env_vlift_fix0; auto.
+      * revert H2; apply fol_equiv_ext; do 2 f_equal.
+        apply vec_pos_ext; intros p; rew vec; rew fot.
+        rewrite env_vlift_fix0; auto.
+    + intros H x y.
+      rewrite fol_sem_mforall; intros v.
+      specialize (H v x y); simpl in H.
+      simpl.
+      rewrite env_vlift_fix1 with (k := 1).
+      rewrite env_vlift_fix1 with (k := 0).
+      rewrite HM; simpl.
+      intros H1 H2; apply H.
+      * revert H1; apply fol_equiv_ext; do 2 f_equal.
+        apply vec_pos_ext; intros p; rew vec; rew fot.
+        rewrite env_vlift_fix0; auto.
+      * revert H2; apply fol_equiv_ext; do 2 f_equal.
+        apply vec_pos_ext; intros p; rew vec; rew fot.
+        rewrite env_vlift_fix0; auto.
+  Qed.
+ 
+  Definition fol_rel_tot (s : syms Σ) : 𝔽' := 
+       let n := ar_syms _ s
+       in fol_mquant fol_fa n (∃ fol_atom Σ' (inl s) (£0##vec_set_pos (fun p => £(1+pos2nat p)))). 
+
+  Fact fol_rel_tot_spec s φ : fol_sem M φ (fol_rel_tot s) <-> graph_tot (fun v x => fom_rels M (inl s) (x##v)).
+  Proof.
+    unfold fol_rel_tot.
+    rewrite fol_sem_mforall.
+    apply forall_equiv; intros v; simpl.
+    apply exists_equiv; intros x.
+    apply fol_equiv_ext; do 2 f_equal.
+    apply vec_pos_ext; intros p; rew vec; rew fot.
+    simpl; rewrite env_vlift_fix0; auto.
+  Qed.
+
+  Definition fol_rels_are_functions ls := fol_lconj (map (fun s => fol_rel_fun s ⟑ fol_rel_tot s) ls).
+
+  Fact fol_rels_are_functions_spec ls φ : 
+         fol_sem M φ (fol_rels_are_functions ls) <-> forall s, In s ls -> is_graph_function (fun v x => fom_rels M (inl s) (x##v)).
+  Proof.
+    unfold fol_rels_are_functions.
+    rewrite fol_sem_lconj; split.
+    + intros H s Hs; red.
+      rewrite <- fol_rel_tot_spec with (φ := φ).
+      rewrite <- fol_rel_fun_spec with (φ := φ).
+      apply (H (fol_rel_fun s ⟑ fol_rel_tot s)), in_map_iff.
+      exists s; auto.
+    + intros H B; rewrite in_map_iff.
+      intros (s & <- & Hs); split.
+      * apply fol_rel_fun_spec, H; auto.
+      * apply fol_rel_tot_spec, H; auto.
+  Qed.
+
+  Definition Σsyms_Σnosyms ls A := fol_rels_are_functions ls ⟑ fol_rem_syms A.
 
 End Sig_remove_symbols.
+
+Theorem Σsyms_Σnosyms_sound Σ ls A X : 
+             @fo_form_fin_discr_dec_SAT_in Σ A X
+          -> @fo_form_fin_dec_eq_SAT_in (fos_nosyms Σ) (inr (inl tt)) (Σsyms_Σnosyms ls A) X.
+Proof.
+  intros (H0 & M & H1 & H2 & phi & H3).
+  exists (fom_nosyms M), H1; destruct M as (sy,re).
+  exists.
+  { intros [s|[[]|r]]; simpl.
+    + intros; apply H0.
+    + intros; apply H0.
+    + intros; apply H2. }
+  exists eq_refl, eq_refl, phi.
+  unfold Σsyms_Σnosyms; split.
+  + apply fol_rels_are_functions_spec; auto.
+    intros s Hs; split.
+    * intros v x y; simpl; intros; subst; auto.
+    * intros v; exists (sy s v); simpl; auto.
+  + revert H3; apply fol_rem_syms_spec.
+Qed.
+
+Section completeness.
+
+  Variable (Σ : fo_signature) (ls : list (syms Σ)) (A : fol_form Σ) 
+           (Hls : forall s, { In s ls } + { ~ In s ls })
+           (HAls : incl (fol_syms A) ls).
+
+  Notation Σ' := (fos_nosyms Σ).
+
+  Let e : rels Σ' := inr (inl tt).
+
+  Variable (X : Type).
+
+  Section nested.
+
+    Variable (M : fo_model Σ' X)  
+             (Xfin : finite_t X) 
+             (Mdec : fo_model_dec M) 
+             (He : fom_rels M e = rel2_on_vec eq)
+             (φ : nat -> X) 
+             (HM : fol_sem M φ (Σsyms_Σnosyms ls A)).
+
+    Let HF : forall s, In s ls -> is_graph_function (fun v x => fom_rels M (inl s) (x##v)).
+    Proof. 
+      simpl in HM; apply proj1 in HM. 
+      rewrite fol_rels_are_functions_spec in HM; auto.
+    Qed.
+
+    Let HA : fol_sem M φ (fol_rem_syms A).
+    Proof. simpl in HM; apply proj2 in HM; auto. Qed.
+
+    Let F (s : syms Σ) : In s ls -> { f | forall v x, fom_rels M (inl s) (x##v) <-> x = f v }.
+    Proof. intro; apply graph_tot_reif; auto. Qed.
+
+    Local Definition Σsyms_Σnosyms_rev_model : fo_model Σ X.
+    Proof.
+      split.
+      + intros s.
+        destruct (Hls s) as [ H | H ].
+        * exact (proj1_sig (F s H)).
+        * exact (fun _ => φ 0).
+      + intros r.
+        exact (fom_rels M (inr (inr r))).
+    Defined.
+
+    Local Fact Σsyms_Σnosyms_complete_nested : fol_sem Σsyms_Σnosyms_rev_model φ A.
+    Proof.
+      apply fol_rem_syms_spec.
+      revert HA.
+      apply fo_model_projection' with (i := fun x => x) (j := fun x => x) (ls := nil) 
+             (lr := inr (inl tt) :: map inl (fol_syms A) ++ map (fun r => inr (inr r)) (fol_rels A)); auto.
+      + intros s v [].
+      + intros r v; simpl In; rewrite in_app_iff, in_map_iff, in_map_iff.
+        intros [ <- | [ (s & <- & Hs) | (r' & <- & Hr') ] ]; simpl.
+        * fold e; rewrite He; simpl in v |- *.
+          vec split v with x; vec split v with y; simpl; tauto.
+        * destruct (Hls s) as [ H | H ]; try tauto.
+          vec split v with x; simpl.
+          rewrite <- (proj2_sig (F s H) v x).
+          apply fol_equiv_ext; f_equal; f_equal.
+          apply vec_pos_ext; intro; rew vec.
+          destruct H; revert Hs; apply HAls.
+        * apply fol_equiv_ext; f_equal; f_equal.
+          apply vec_pos_ext; simpl; intros; rew vec.
+          rewrite vec_pos_map; auto.
+      + intros [].
+      + apply fol_rem_syms_rels.
+    Qed.
+
+  End nested.
+
+  Theorem Σsyms_Σnosyms_complete : 
+          @fo_form_fin_dec_eq_SAT_in (fos_nosyms Σ) (inr (inl tt)) (Σsyms_Σnosyms ls A) X
+       -> @fo_form_fin_discr_dec_SAT_in Σ A X.
+  Proof.
+    intros (M & H1 & H2 & H3 & H4 & phi & H5).
+    fold e in H3, H4.
+    revert H3 H4; simpl; intros H3.
+    rewrite eq_nat_pirr with (H := H3); simpl.
+    clear H3; intros H4.
+    exists.
+    { intros x y.
+      generalize (H2 e (x##y##ø)).
+      rewrite H4; simpl; tauto. }
+    exists (Σsyms_Σnosyms_rev_model H1 H2 H4 H5).
+    exists H1.
+    exists.
+    { intros r v; simpl; apply H2. }
+    exists phi.
+    apply Σsyms_Σnosyms_complete_nested.
+  Qed.
+
+End completeness.
+ 
+Check Σsyms_Σnosyms_sound.
+Check Σsyms_Σnosyms_complete. 
